TPTP/Render.lean
@@ -8,19 +8,27 @@ import TPTP.Syntax
 
 namespace TPTP
 
-def Statement.render (statement : Statement) : String :=
+def Statement.render
+    (statement : Statement)
+    : String :=
   let annotation := statement.annotations.map (fun value => s!", {value}") |>.getD ""
   s!"{statement.kind}({statement.name}, {statement.role}, {statement.formula}{annotation})."
 
-def Include.render (value : Include) : String :=
+def Include.render
+    (value : Include)
+    : String :=
   let selection := value.selection.map (fun item => s!", {item}") |>.getD ""
   s!"include({value.path}{selection})."
 
-def Item.render : Item → String
+def Item.render
+    : Item →
+      String
   | .statement value => value.render
   | .include value => Include.render value
 
-def Document.render (document : Document) : String :=
+def Document.render
+    (document : Document)
+    : String :=
   String.intercalate "\n" (document.items.toList.map Item.render)
 
 end TPTP
